examples/graph/module-edits/Data/Graph/Inductive/Query/BFS/midamble.v
@@ -3,3 +3,28 @@ Instance LPath__Default {a} : GHC.Err.Default (Data.Graph.Inductive.Graph.LPath 
 
 Instance Queue__Default {a} : GHC.Err.Default (Data.Graph.Inductive.Internal.Queue.Queue a) :=
   { default := Data.Graph.Inductive.Internal.Queue.MkQueue nil nil }.
+
+(*Need to rewrite this because of laziness issue - We cannot call queueGet before knowing that the queue is non-empty*)
+Definition bf {gr} {a} {b} `{(Data.Graph.Inductive.Graph.Graph gr)}
+   : Data.Graph.Inductive.Internal.Queue.Queue Data.Graph.Inductive.Graph.Path ->
+     gr a b -> Data.Graph.Inductive.Internal.RootPath.RTree :=
+  GHC.DeferredFix.deferredFix2 (fun bf
+                                (q : Data.Graph.Inductive.Internal.Queue.Queue Data.Graph.Inductive.Graph.Path)
+                                (g : gr a b) =>
+                                 if orb (Data.Graph.Inductive.Internal.Queue.queueEmpty q)
+                                             (Data.Graph.Inductive.Graph.isEmpty g) : bool
+                                      then nil else
+                                  match Data.Graph.Inductive.Internal.Queue.queueGet q with
+                                  | pair (cons v _ as p) q' =>
+                                      match Data.Graph.Inductive.Graph.match_ v g with
+                                      | pair (Some c) g' =>
+                                          cons p (bf (Data.Graph.Inductive.Internal.Queue.queuePutList (GHC.Base.map
+                                                                                                        (fun arg_2__ =>
+                                                                                                           cons arg_2__
+                                                                                                                p)
+                                                                                                        (Data.Graph.Inductive.Graph.suc'
+                                                                                                         c)) q') g')
+                                      | pair None g' => bf q' g'
+                                      end
+                                  | _ => GHC.Err.patternFailure
+                                  end).
